Significant step towards a fully functional tree-based refinement
Rewrote the entire tree-based example to use the new nested trees
framework. Observers are fully refined and proved, while some parts of
the mutators are still admitted.

In the process, the dual list/tree structure that the example was
previously using was unified into a single nested tree structure, and
the State inductive types was replaced with nats (though it could
possibly use bounded strings in the future). As a consequence, the list-
based example was removed from the Makefile.

ADTExamples/QueryStructure/ProcessScheduler/TreeBasedRefinement.v
@@ -1,131 +1,83 @@
-Require Import List Omega Ensembles.
+Require Import String Omega List FunctionalExtensionality Ensembles
+        Computation ADT ADTRefinement ADTNotation BuildADTRefinements
+        QueryStructureSchema QueryStructure
+        QueryQSSpecs InsertQSSpecs EmptyQSSpecs
+        GeneralInsertRefinements GeneralQueryRefinements
+        GeneralQueryStructureRefinements
+        ListQueryRefinements ListInsertRefinements
+        ListQueryStructureRefinements
+        ProcessScheduler.AdditionalLemmas
+        DBSchema SetEq.
 
+Require Import Bags.
 Require Import FMapAVL OrderedTypeEx.
 Require Import FMapExtensions.
 Require Import DBSchema SetEq AdditionalLemmas.
 Require Export ADTRefinement.BuildADTRefinements.
 
-Require Import GeneralInsertRefinements ListInsertRefinements
-        GeneralQueryRefinements ListQueryRefinements.
-
 Unset Implicit Arguments.
 
 Module GenericTreeDB := FMapAVL.Make(Nat_as_OT). (* TODO: Add the generic implementation *)
-Module Import DBExtraFacts := FMapExtensions GenericTreeDB.
+(*Module Import DBExtraFacts := FMapExtensions GenericTreeDB.*)
+
+Definition PIDIndex : BagPlusBagProof ProcessSchema.
+Proof.
+  mkIndex ProcessSchema [STATE; PID].
+Defined.
+
+Definition PIDIndexedTree := BagType _ PIDIndex.
 
 Section TreeBasedRefinement.
   Open Scope type_scope.
   Open Scope Tuple_scope.
 
-  Definition TreeDB : Type := GenericTreeDB.t Process.
-
   Definition NeatDB :=
-    (nat * (TreeDB * TreeDB)).
-
-  Definition AllSleepingSet ensemble :=
-    fun (p: Process) => ensemble p /\ p!STATE = Sleeping.
-
-  Definition AllRunningSet ensemble :=
-    fun (p: Process) => ensemble p /\ p!STATE = Running.
-
-  Definition KeyedOnPID (tree: TreeDB) :=
-    forall (p: Process),
-      forall (a: nat),
-        GenericTreeDB.MapsTo a p tree ->
-        a = p!PID.
-
-  Lemma KeyedOnPID_add :
-    forall process tree pid,
-      KeyedOnPID tree ->
-      process!PID = pid ->
-      KeyedOnPID (GenericTreeDB.add pid process tree).
-  Proof.
-    unfold KeyedOnPID; intros.
-    rewrite add_mapsto_iff in H1.
-    destruct H1;
-      intuition;
-      subst; intuition.
-  Qed.
+    (nat * PIDIndexedTree).
 
   Definition NeatDB_equivalence old_rep (neat_db: NeatDB) :=
-    let (next_pid, databases) := neat_db in
+    (*TODO: Would be cleaner: let (next_pid, database) := neat_db in*)
     let set_db := GetUnConstrRelation old_rep PROCESSES in
-    (forall pid, (forall tuple, In _ set_db tuple -> tuple!PID = pid -> lt pid next_pid))
-    /\
-    (let (sleeping, running) := databases in
-     (EnsembleListEquivalence (AllSleepingSet set_db) (GetValues sleeping) /\
-      KeyedOnPID sleeping)
-     /\
-     (EnsembleListEquivalence (AllRunningSet  set_db) (GetValues running ) /\
-      KeyedOnPID running)).
+    (forall tuple, In _ set_db tuple -> gt (fst neat_db) (tuple PID)) /\
+    (EnsembleListEquivalence set_db (benumerate (snd neat_db))).
+
+  Definition ObservationalEq {A B} f g :=
+    forall (a: A), @eq B (f a) (g a).
+
+  Lemma filter_by_equiv :
+    forall {A} f g,
+      ObservationalEq f g ->
+      forall seq, @List.filter A f seq = @List.filter A g seq.
+  Proof.
+    intros A f g obs seq; unfold ObservationalEq in obs; induction seq; simpl; try rewrite obs; try rewrite IHseq; trivial.
+  Qed.
 
   Lemma filter_on_key :
-    forall (tree: TreeDB)
-           (equality: nat -> nat -> bool)
-           (equality_iff: forall x y, equality x y = true <-> x = y),
-    forall (key: nat),
-      KeyedOnPID tree ->
+    forall (tree: PIDIndexedTree) (key: nat),
       SetEq
         (List.filter
-           (fun (p: Process) => equality (p!PID) key)
-           (GetValues tree))
-        (Option2Box
-           (GenericTreeDB.find key tree)).
+           (fun (p: Process) => beq_nat (p PID) key)
+           (benumerate tree))
+        (bfind tree (None, (Some key, bstar))).
   Proof.
-    unfold KeyedOnPID.
-    unfold SetEq, GetValues.
-    intros; intuition.
+    intros tree key.
 
-    rewrite in_Option2Box.
-    rewrite filter_In in *.
-    rewrite in_map_iff in *.
-    destruct H0 as ([x0 (_snd, in_seq)], _fst).
-    unfold dec2bool in *.
-
-    rewrite <- find_mapsto_iff.
-    destruct x0.
-    subst; simpl in *.
-    apply in_elements_mapsto in in_seq.
-
-    specialize (H p k in_seq).
-
-    rewrite equality_iff in *.
-    subst; trivial.
-
-    (****)
-
-    rewrite in_Option2Box in H0.
-    rewrite filter_In in *.
-    unfold dec2bool in *.
-    rewrite <- find_mapsto_iff in H0.
-    pose proof H0 as H2.
-    rewrite elements_mapsto_iff in H0.
-    apply InA_In_snd in H0.
-    intuition.
-
-    specialize (H x key H2).
-
-    rewrite equality_iff in *.
-    intuition.
+    rewrite (filter_by_equiv _ (@bfind_matcher _ _ _ (BagProof _ PIDIndex) (None, (Some key, bstar)))).
+    apply (bfind_correct).
+    
+    unfold ObservationalEq.
+    simpl.
+    intros.
+    rewrite (NatTreeExts.KeyFilter_beq beq_nat) by apply NPeano.Nat.eqb_spec.
+    rewrite andb_true_r; unfold cast; trivial.
   Qed.
 
   Notation "x '∈' y" := (In _ y x) (at level 50, no associativity).
-
-  Lemma partition_set :
-    forall ens x,
-      (fun x => AllRunningSet ens x \/ AllSleepingSet ens x) x <-> ens x.
-  Proof.
-    unfold AllRunningSet, AllSleepingSet;
-    intros ens x;
-    destruct (x!STATE);
-      tauto.
-  Qed.
 
   Lemma no_collisions_when_using_a_fresh_pid :
     forall pid c (tup tup': Process),
       tupleAgree tup tup' [PID_COLUMN]%SchemaConstraints ->
       (forall a, (GetUnConstrRelation c PROCESSES) a -> pid > (a PID)) ->
-      tup!PID = pid ->
+      tup PID = pid ->
       GetUnConstrRelation c PROCESSES tup' ->
       False.
   Proof.
@@ -147,10 +99,10 @@ Section TreeBasedRefinement.
                  (forall tup' : Tuple,
                     GetUnConstrRelation c PROCESSES tup' ->
                     tupleAgree
-                      (<PID_COLUMN :: pid, STATE_COLUMN :: Sleeping, CPU_COLUMN :: 0>) tup'
+                      (<PID_COLUMN :: pid, STATE_COLUMN :: SLEEPING, CPU_COLUMN :: 0>) tup'
                       [PID_COLUMN]%SchemaConstraints ->
                     tupleAgree
-                      (<PID_COLUMN :: pid, STATE_COLUMN :: Sleeping, CPU_COLUMN :: 0>) tup'
+                      (<PID_COLUMN :: pid, STATE_COLUMN :: SLEEPING, CPU_COLUMN :: 0>) tup'
                       [CPU_COLUMN; STATE_COLUMN]%SchemaConstraints)
                     }
         (ret true).
@@ -176,10 +128,10 @@ Section TreeBasedRefinement.
                  (forall tup' : Tuple,
                     GetUnConstrRelation c PROCESSES tup' ->
                     tupleAgree
-                      tup' (<PID_COLUMN :: pid, STATE_COLUMN :: Sleeping, CPU_COLUMN :: 0>)
+                      tup' (<PID_COLUMN :: pid, STATE_COLUMN :: SLEEPING, CPU_COLUMN :: 0>)
                       [PID_COLUMN]%SchemaConstraints ->
                     tupleAgree
-                      tup' (<PID_COLUMN :: pid, STATE_COLUMN :: Sleeping, CPU_COLUMN :: 0>)
+                      tup' (<PID_COLUMN :: pid, STATE_COLUMN :: SLEEPING, CPU_COLUMN :: 0>)
                       [CPU_COLUMN; STATE_COLUMN]%SchemaConstraints)
                     }
         (ret true).
@@ -188,15 +140,15 @@ Section TreeBasedRefinement.
     intros; exfalso; rewrite tupleAgree_sym in H1; apply (no_collisions_when_using_a_fresh_pid pid c _ _ H1); trivial.
   Qed.
 
+(*
   Lemma refine_pick_fmap_add_matching :
     forall tree ens tuple pid (cond: Process -> Prop),
       cond tuple ->
-      tuple!PID = pid ->
-      KeyedOnPID tree ->
+      tuple PID = pid ->
       (~ GenericTreeDB.In (elt:=Tuple) pid tree) ->
       (EnsembleListEquivalence
          (fun tuple' => In _ (GetUnConstrRelation ens PROCESSES) tuple' /\ cond tuple')
-         (GetValues tree)) ->
+         (benumerate tree)) ->
       refine
         {a |
          EnsembleListEquivalence
@@ -206,8 +158,7 @@ Section TreeBasedRefinement.
                          ProcessSchedulerSchema ens PROCESSES
                          (RelationInsert tuple (GetUnConstrRelation ens PROCESSES)))
                       PROCESSES) tuple' /\ cond tuple')
-           (GetValues a) /\
-         KeyedOnPID a}
+           (benumerate a)}
         (ret (GenericTreeDB.add pid tuple tree)).
   Proof.
     unfold refine;
@@ -292,170 +243,194 @@ Section TreeBasedRefinement.
     pose proof (H _ _ ina); subst.
     eauto.
   Qed.
-
+*)
 
   Lemma NeatScheduler :
     Sharpened ProcessSchedulerSpec.
   Proof.
-    hone representation using (@DropQSConstraints_SiR ProcessSchedulerSchema).
+    unfold ProcessSchedulerSpec.
 
-    hone mutator SPAWN.
-    {
-      unfold ForAll_In. (*TODO: Why does swapping these two calls break 'finish honing'?*)
-      remove trivial insertion checks.
+    unfold ForAll_In; start honing QueryStructure.
+
+    hone representation using NeatDB_equivalence.
+    
+    (* (* TODO: Why does adding this followed simpl break the 
+          Equivalent_UnConstr_In_EnsembleListEquivalence rewrite? *) 
+      unfold UnConstrQuery_In.
+     (*simpl.*) *)
+
+    hone constructor INIT. {
+      unfold NeatDB_equivalence, DropQSConstraints_SiR.
+      repeat setoid_rewrite refineEquiv_pick_ex_computes_to_and.
+      repeat setoid_rewrite refineEquiv_pick_eq'.
+      simplify with monad laws.
+
+      setoid_rewrite (* TODO *)
+        (refineEquiv_pick_pair_snd_dep
+           (fun frist => forall tuple : Tuple, tuple ∈ _ -> frist > tuple PID)
+           (fun pair  => EnsembleListEquivalence _ (benumerate (snd pair)))).
+
+      rewrite refine_pick_val;
+        [ simplify with monad laws | instantiate (1 := 0) ].
+
+      rewrite refine_pick_val;
+        [ simplify with monad laws | instantiate (1 := bempty); apply EnsembleListEquivalence_Empty ].
+
+      subst_body; higher_order_1_reflexivity. (* TODO: finish constructing? *)
+
+      (* Buffered pid value correct *)
+      intros tuple in_empty;
+      apply EnsembleListEquivalence_Empty in in_empty;
+      intuition.
+    }
+
+    hone method ENUMERATE. {
+      pose proof H;
+      unfold NeatDB_equivalence in H;
+      destruct H as (next_pid_correct & db_equiv);
+      simpl Domain in next_pid_correct.
+
+      setoid_rewrite refineEquiv_pick_ex_computes_to_and.
+      setoid_rewrite refineEquiv_pick_pair.
+      setoid_rewrite refineEquiv_pick_eq'. 
+      simplify with monad laws.
+      simpl.
+
+      rewrite (Equivalent_UnConstr_In_EnsembleListEquivalence);
+        eauto. (* TODO: Could explicitly pass the right list *)
+
+      setoid_rewrite Equivalent_List_In_Where.
+
+      rewrite (filter_by_equiv dec (bfind_matcher (Some n, (None, []))))
+        by (
+            unfold ObservationalEq; simpl; 
+            unfold NatTreeExts.KeyFilter;
+            unfold NatTreeExts.MoreFacts.BasicProperties.F.eq_dec;
+            
+            intros;
+            rewrite ?andb_true_r, ?andb_true_l;
+            intuition
+          ).
+
+      setoid_rewrite (@bfind_correct _ _ _ (BagProof _ PIDIndex) (snd r_n) (Some n, (None, []))).
+      setoid_rewrite refine_For_List_Return.
+      simplify with monad laws.
+
+      rewrite refine_pick_val by eassumption.
+      simplify with monad laws.
+      finish honing.
+    }    
+
+    (* TODO: s/Decideable/Decidable/ *)
+    (* TODO: Use rewrite by instead of [ ... | eassumption ] *)
+    (* TODO: Handle the 'projection' parameter differently; 
+             right now it appears explicitly in plenty of 
+             places, and since it is infered in KeyFilter 
+             it makes it possble to swap same-type search terms,
+             delaying the failure until the call to bfind_correct *)
+    (* TODO: The backtick notation from bounded indexes cannot be input *)
+    (* TODO: The call to filter_by_equiv generates existentials, probably 
+             corresponding to projections *)
+   
+    hone method GET_CPU_TIME. {
+      pose proof H;
+      unfold NeatDB_equivalence in H;
+      destruct H as (next_pid_correct & db_equiv);
+      simpl Domain in next_pid_correct.
+      
+      setoid_rewrite refineEquiv_pick_ex_computes_to_and.
+      setoid_rewrite refineEquiv_pick_pair.
+      setoid_rewrite refineEquiv_pick_eq'. 
+      simplify with monad laws.
+      simpl.
+
+      rewrite (Equivalent_UnConstr_In_EnsembleListEquivalence);
+        eauto. (* TODO: Could explicitly pass the right list *)
+
+      setoid_rewrite Equivalent_List_In_Where.
+      rewrite (filter_by_equiv dec (bfind_matcher (None, (Some n, [])))) 
+        by (
+            unfold ObservationalEq; simpl; 
+            unfold NatTreeExts.KeyFilter;
+            unfold NatTreeExts.MoreFacts.BasicProperties.F.eq_dec;
+            
+            intros;
+            rewrite ?andb_true_r, ?andb_true_l;
+            intuition
+          ).
+      setoid_rewrite (@bfind_correct _ _ _ (BagProof _ PIDIndex) (snd r_n) (None, (Some n, []))).
+      setoid_rewrite refine_For_List_Return.
+      simplify with monad laws.
+
+      rewrite refine_pick_val by eassumption.
+      simplify with monad laws.
       finish honing.
     }
 
-    hone representation using NeatDB_equivalence.
+    hone method SPAWN. {
+      pose proof H;
+      unfold NeatDB_equivalence in H;
+      destruct H as (next_pid_correct & db_equiv);
+      simpl Domain in next_pid_correct.
+      
+      setoid_rewrite refineEquiv_pick_ex_computes_to_and.
+      setoid_rewrite refineEquiv_pick_pair.
+      setoid_rewrite refineEquiv_pick_eq'. 
+      simplify with monad laws.
+      simpl.
+ 
+      rewrite refine_pick_val by eassumption.
+      simplify with monad laws.
 
-    hone_observer' ENUMERATE.
+      rewrite refine_pick_val;
+        [ | instantiate (1 := true) ].
+      simplify with monad laws.
 
-    intros db state result computes set_db_unconstr set_db constr_unconstr_equiv db_equiv.
+      rewrite refine_pick_val;
+        [ | instantiate (1 := true) ].
+      simplify with monad laws.
 
-    destruct db as (next_pid & sleeping & running);
-      unfold NeatDB_equivalence in db_equiv;
-      destruct db_equiv as (nextpid_correct & (sleeping_correct & sleeping_keys)
-                                            & (running_correct & running_keys)).
+      unfold NeatDB.
+      simpl.
 
-    pose proof (equiv_EnsembleListEquivalence
-                  (partition_set (GetUnConstrRelation set_db_unconstr PROCESSES))
-                  (SetUnion_Or running_correct sleeping_correct)).
+      unfold NeatDB_equivalence.
+      simpl Domain.
+      
+      setoid_rewrite 
+        (refineEquiv_pick_pair_snd_dep
+           (fun frist => forall tuple : Tuple, tuple ∈ _ -> frist > tuple PID)
+           (fun pair  => EnsembleListEquivalence _ (benumerate (snd pair)))).
 
-    unfold DropQSConstraints_SiR in constr_unconstr_equiv.
-    pose proof H.
-    rewrite <- constr_unconstr_equiv, GetRelDropConstraints in H.
+      simplify with monad laws.
 
-    set (full_db := SetUnion (GetValues running) (GetValues sleeping)).
+      rewrite refine_pick_val;
+        [ | instantiate (1 := S (fst r_n)) ].
+      simplify with monad laws.      
 
-    unfold EnsembleListEquivalence, In, AllRunningSet, AllSleepingSet
-      in sleeping_correct, running_correct.
+      rewrite refine_pick_val;
+        [ | instantiate (1 := (binsert (snd r_n) <PID_COLUMN :: S (fst r_n), STATE_COLUMN :: SLEEPING, CPU_COLUMN :: 0>))].
 
-    symmetry in sleeping_correct, running_correct.
+      simplify with monad laws.
 
-    rewrite (refine_ensemble_into_list full_db _ _ _ (fun p => beq_state p!STATE Running))
-      in running_correct;
-      eauto using beq_process_iff__state.
+      finish honing.
 
-    rewrite (refine_ensemble_into_list full_db _ _ _ (fun p => beq_state p!STATE Sleeping))
-      in sleeping_correct;
-      eauto using beq_process_iff__state.
+      (* Insert correct -- should be in the signature *)
+      admit.
 
-    rewrite (refine_ensemble_into_list_with_extraction full_db _ _ _ (fun p => beq_state p!STATE state));
-      eauto using beq_process_iff__state.
+      (* Buffered value for next_pid correct *)
+      unfold In, GetUnConstrRelation, UpdateUnConstrRelation, RelationInsert in next_pid_correct |- *;
+      simpl in next_pid_correct |- *;
+      intros tuple [ is_new | is_old ]; 
+        [ subst | apply lt_S ];
+        intuition.
 
-    rewrite (state_eta_rule state (fun l => map _ _) (fun x => SetEq result x)).
-
-    rewrite <- sleeping_correct, <- running_correct.
-
-    rewrite <- !map_list_map_fmap.
-
-    refine_eq_into_ret.
-
-    pull_definition.
-
-    hone_observer' GET_CPU_TIME.
-
-    intros db pid result computes set_db_unconstr set_db constr_unconstr_equiv db_equiv.
-
-    destruct db as (next_pid & sleeping & running);
-      unfold NeatDB_equivalence in db_equiv;
-      destruct db_equiv as (nextpid_correct & (sleeping_correct & sleeping_keys)
-                                            & (running_correct & running_keys)).
-
-    pose proof (equiv_EnsembleListEquivalence
-                  (partition_set (GetUnConstrRelation set_db_unconstr PROCESSES))
-                  (SetUnion_Or running_correct sleeping_correct)).
-
-    unfold DropQSConstraints_SiR in constr_unconstr_equiv.
-    pose proof H.
-    rewrite <- constr_unconstr_equiv, GetRelDropConstraints in H.
-
-    set (full_db := SetUnion (GetValues running) (GetValues sleeping)).
-
-    unfold EnsembleListEquivalence, In, AllRunningSet, AllSleepingSet
-      in sleeping_correct, running_correct.
-    symmetry in sleeping_correct, running_correct.
-
-    rewrite (refine_ensemble_into_list full_db _ _ _ (fun p => beq_state p!STATE Running))
-      in running_correct;
-      eauto using beq_process_iff__state.
-
-    rewrite (refine_ensemble_into_list full_db _ _ _ (fun p => beq_state p!STATE Sleeping))
-      in sleeping_correct;
-      eauto using beq_process_iff__state.
-
-    rewrite (refine_ensemble_into_list_with_extraction full_db _ _ _ (fun p => beq_nat p!PID pid));
-      eauto using beq_process_iff__pid.
-
-    unfold full_db;
-      rewrite filter_union.
-
-    repeat rewrite filter_on_key;
-      eauto using beq_nat_true_iff.
-
-    refine_eq_into_ret.
-
-    pull_definition.
-
-    hone mutator SPAWN.
-
-    unfold NeatDB_equivalence, NeatDB in *;
-      destruct r_n as (next_pid & sleeping & running);
-      destruct H as (nextpid_correct & (sleeping_correct & sleeping_keys)
-                                     & (running_correct & running_keys));
-      simpl in *.
-
-    setoid_rewrite refineEquiv_split_ex.
-    setoid_rewrite refineEquiv_pick_computes_to_and.
-    simplify with monad laws.
-
-    setoid_rewrite (refine_pick_val _ (a := next_pid)); eauto.
-    simplify with monad laws.
-    setoid_rewrite insert_always_happens; eauto.
-    simplify with monad laws.
-    setoid_rewrite insert_always_happens'; eauto.
-    simplify with monad laws.
-    setoid_rewrite refine_pick_eq_ex_bind.
-
-    setoid_rewrite refine_let.
-    setoid_rewrite (refine_pick_val _ (a := S next_pid)).
-
-    simplify with monad laws.
-    setoid_rewrite refine_let.
-
-    simplify with monad laws.
-    setoid_rewrite (refine_pick_fmap_add_matching sleeping _ _ _ (fun x => x!STATE = Sleeping)); eauto.
-    simplify with monad laws.
-    setoid_rewrite (refine_pick_fmap_add_not_matching running _ _ (fun x => x!STATE = Running)); eauto.
-    simplify with monad laws.
-
-    apply refine_ret_eq.
-    unfold H0; clear H0.
-    pull_definition.
-
-    (* Didn't insert a running process *)
-    discriminate.
-
-    (* No duplicates *)
-
-    unfold not; intro has_key.
-    apply In_InValues in has_key; eauto.
-    destruct has_key as [tup (collision & already_inserted)].
-    unfold EnsembleListEquivalence in sleeping_correct;
-      rewrite <- sleeping_correct in already_inserted.
-
-    apply weaken, (nextpid_correct tup!PID) in already_inserted; eauto.
-    compute in collision, already_inserted.
-    omega.
-
-    (* Updated next_pid properly *)
-    unfold In, GetUnConstrRelation, UpdateUnConstrRelation, RelationInsert in *;
-      simpl in *;
-      intros pid tuple [ is_new_process | is_updated_process ] pid_eq;
-      subst;
-      [ compute | apply lt_S, (nextpid_correct _ tuple) ];
-      intuition.
+      (* Unicity constraints respected *)
+      admit.
+      admit.      
+    }
 
     finish sharpening.
+
+    Grap Existential Variables. (* TODO: This returns 'no such unproven subgoal' :/ *)
   Defined.
 End TreeBasedRefinement.
